extend adaptation

Probabilities.thy
@@ -120,7 +120,7 @@ next
 section "Use the unit interval to model probabilities"
 
 
-interpretation PROB: quant_sep_con  "( * )"   "one_unitinterval"   "divide_unitinterval"
+interpretation PROB: quant_sep_con  Inf Sup inf "(\<le>)" "(<)" sup top bot "( * )"   "one_unitinterval"   "divide_unitinterval"
   apply (standard; transfer)
   subgoal by (auto simp: algebra_simps min_absorb1 divide_ereal_def) 
   subgoal by (auto simp: algebra_simps min_absorb1 divide_ereal_def) 
@@ -148,11 +148,8 @@ interpretation PROB: quant_sep_con  "( * )"   "one_unitinterval"   "divide_uniti
 
 
 
-abbreviation star_prob (infixl "**\<^sub>w" 60) where
-  "star_prob == PROB.sep_conj_q"
-
-abbreviation wand_prob (infixl "-*\<^sub>w" 60) where
-  "wand_prob == PROB.sep_impl_qq"
+definition star_prob (infixl "**\<^sub>w" 60) where "star_prob == PROB.sep_conj_q"
+definition wand_prob (infixl "-*\<^sub>w" 60) where "wand_prob == PROB.sep_impl_qq"
 
 
 
@@ -163,33 +160,33 @@ lemma times_fun': "f * g = (\<lambda>h. f h * g h)"
 subsubsection \<open>Star and Magic Wand with State\<close>
 
 
-abbreviation sep_conj_us (infixr "\<star>\<^sub>u" 35) where "sep_conj_us == PROB.sep_conj_s_q"
-abbreviation sep_impl_us (infixr "-\<star>\<^sub>u" 35) where "sep_impl_us == PROB.sep_impl_s_q"
-abbreviation "sep_empty_s\<^sub>u \<equiv> PROB.sep_empty_s_q" 
-abbreviation "emb\<^sub>u \<equiv> PROB.emb" 
+definition sep_conj_us (infixr "\<star>\<^sub>u" 35) where "sep_conj_us == PROB.sep_conj_s_q"
+definition sep_impl_us (infixr "-\<star>\<^sub>u" 35) where "sep_impl_us == PROB.sep_impl_s_q"
+definition "sep_empty_s\<^sub>u \<equiv> PROB.sep_empty_s_q" 
+definition "emb\<^sub>u \<equiv> PROB.emb" 
 
-lemma sep_conj_es_def:
+lemma sep_conj_us_alt:
   fixes P :: "(_ \<times> 'a::{sep_algebra} \<Rightarrow> unitinterval)"
   shows "(P \<star>\<^sub>u Q) = (\<lambda>(s,h). Sup { P(s,x) * Q(s,y) | x y. h=x+y \<and> x ## y})"
-  by (simp add: PROB.sep_conj_s_q_def PROB.sep_conj_q_def)
+  by (simp add: PROB.sep_conj_s_q_def PROB.sep_conj_q_def sep_conj_us_def)
 
 term sep_impl_us
 
-lemma sep_impl_es_def:
+lemma sep_impl_us_alt:
   "(P -\<star>\<^sub>u Q) = (\<lambda>(s,h). INF h': { h'. h ## h' \<and> (bot < P(s,h') \<or> bot < Q(s,h+h') )
                                 \<and> ( P(s,h') < top \<or> Q(s,h+h') < top)}. 
                                    Q (s,h + h') /\<^sub>u P (s,h') )"
-  by (simp add: PROB.sep_impl_qq_def PROB.sep_impl_s_q_def )
+  by (simp add: PROB.sep_impl_qq_def PROB.sep_impl_s_q_def  sep_impl_us_def)
 
-lemma sep_empty_s\<^sub>u_def: "sep_empty_s\<^sub>u = (\<lambda>(s, y). emb\<^sub>u (\<lambda>h. h = 0) y)"
-  by (auto simp: PROB.sep_empty_s_q_def PROB.sep_empty_q_def  )
+lemma sep_empty_s\<^sub>u_alt: "sep_empty_s\<^sub>u = (\<lambda>(s, y). emb\<^sub>u (\<lambda>h. h = 0) y)"
+  by (auto simp: PROB.sep_empty_s_q_def PROB.sep_empty_q_def emb\<^sub>u_def sep_empty_s\<^sub>u_def )
 
-lemmas sep_conj_es_commute =  PROB.sep_conj_s_q_commute
-lemmas sep_conj_es_neutral = PROB.sep_conj_s_q_neutral
-lemmas sep_conj_es_assoc = PROB.sep_conj_s_q_assoc
-lemmas sep_conj_es_left_commute_s = PROB.sep_conj_q_left_commute_s
+lemmas sep_conj_es_commute =  PROB.sep_conj_s_q_commute[folded sep_conj_us_def]
+lemmas sep_conj_es_neutral = PROB.sep_conj_s_q_neutral[folded sep_conj_us_def sep_empty_s\<^sub>u_def]
+lemmas sep_conj_es_assoc = PROB.sep_conj_s_q_assoc[folded sep_conj_us_def]
+lemmas sep_conj_es_left_commute_s = PROB.sep_conj_q_left_commute_s[folded sep_conj_us_def]
 
-lemmas sep_conj_es_c = PROB.sep_conj_q_s_c
+lemmas sep_conj_es_c = PROB.sep_conj_q_s_c[folded sep_conj_us_def]
 
 
 lemma theorem_3_6_s:
@@ -198,39 +195,43 @@ lemma theorem_3_6_s:
   "(P \<star>\<^sub>u sup Q R) = (\<lambda>s. sup ((P \<star>\<^sub>u Q) s) ((P \<star>\<^sub>u R) s))"
   (*  "(P \<star> (\<lambda>s. Q s + R s)) \<le> (\<lambda>s. (P \<star> Q) s + (P \<star> R) s)" *)
   "( (emb\<^sub>u \<phi>) \<star>\<^sub>u (Q * R)) \<le> ((emb\<^sub>u \<phi>) \<star>\<^sub>u Q) * ((emb\<^sub>u \<phi>) \<star>\<^sub>u R)"
-  subgoal using PROB.theorem_3_6_s(1) .
+  subgoal using PROB.theorem_3_6_s(1)[folded sep_conj_us_def]
+    unfolding sup_fun_def .
   subgoal
     apply(subst (1) times_fun')    
-    using PROB.theorem_3_6_s(2)
-    by (auto simp: le_fun_def)
+    using PROB.theorem_3_6_s(2)[folded sep_conj_us_def emb\<^sub>u_def]
+     by (auto simp: le_fun_def)
   done
 
-lemmas sep_conj_es_mono = PROB.sep_impl_s_q_mono
-lemmas sep_impl_es_mono = PROB.sep_conj_s_q_mono'
+lemmas sep_conj_es_mono = PROB.sep_impl_s_q_mono[folded sep_impl_us_def emb\<^sub>u_def] 
 
 lemma adjoint_general_s:
   shows "(X \<star>\<^sub>u P) \<le> Y \<longleftrightarrow> X \<le> (P -\<star>\<^sub>u Y)" 
-  using PROB.adjoint_general_s by auto
+  using PROB.adjoint_general_s[folded sep_impl_us_def sep_conj_us_def emb\<^sub>u_def] 
+  unfolding le_fun_def by blast
 
 
 lemma quant_modus_ponens_general_s:
   shows "( P \<star>\<^sub>u (P -\<star>\<^sub>u X)) \<le> X"
-  using PROB.quant_modus_ponens_general_s by auto
+  using PROB.quant_modus_ponens_general_s [folded sep_impl_us_def sep_conj_us_def emb\<^sub>u_def] 
+  unfolding le_fun_def by blast
 
 
-abbreviation "pure\<^sub>u \<equiv> PROB.pure_q"
+definition "pure\<^sub>u \<equiv> PROB.pure_q"
 
-lemma pure\<^sub>u_def: "pure\<^sub>u X \<longleftrightarrow> (\<forall>s h1 h2. X (s,h1) = X (s,h2))"
-  using PROB.pure_q_def .
+lemma pure\<^sub>u_alt: "pure\<^sub>u X \<longleftrightarrow> (\<forall>s h1 h2. X (s,h1) = X (s,h2))"
+  using PROB.pure_q_def unfolding pure\<^sub>u_def .
 
 lemma  theorem_3_11_1: "pure\<^sub>u X \<Longrightarrow> X * Y \<le> (X \<star>\<^sub>u Y)"
     apply(subst (1) times_fun')   
-  using PROB.theorem_3_11_1 by auto
+  using PROB.theorem_3_11_1[folded sep_impl_us_def sep_conj_us_def emb\<^sub>u_def pure\<^sub>u_def] 
+  unfolding le_fun_def by blast
 
 lemma theorem_3_11_3:
   "pure\<^sub>u X \<Longrightarrow> ((X * Y) \<star>\<^sub>u Z) = X * (Y \<star>\<^sub>u Z)"
     apply(subst times_fun')+
-  using PROB.theorem_3_11_3 by auto  
+  using PROB.theorem_3_11_3[folded sep_impl_us_def sep_conj_us_def emb\<^sub>u_def pure\<^sub>u_def] 
+  unfolding le_fun_def by blast 
 
 
 
